Getting to the interesting bit soon

ntor/Security.ec
@@ -249,57 +249,14 @@ module (Red_ROM3_real (D : A_GAKE) (O1 : ROSc.I1.RO) : ROSc.I2.RO_Distinguisher)
   }
 }.
 
-module (Red_ROM4_real (D : A_GAKE) (O1 : ROSc.I1.RO) : ROSc.I2.RO_Distinguisher) (O2 : ROSc.I2.RO) = {
-  module AKE_O : GAKE_out = Game2 with {
-    proc init_mem [
-      ^h1m<- ~ {O1.init();}
-      ^h2m<- -
-    ]
-
-    proc h [ 
-      ^t<$ ~ {t <@ O1.get(x); k <@ O2.get(x);}
-      ^if -
-      ^k<$ -
-      ^if -
-    ] res ~ ((t, k))
-
-    proc send_msg2 [
-      ^match#Some.^match#None.^if.^ts<$ ~ {t_B <@ O1.get(x); sk <@ O2.get(x);}
-      [^match#Some.^match#None.^if.^if - ^sk<-] -
-    ]
-
-    proc send_msg3 [
-      ^match#Some.^match#Pending.^ts<$ ~ {t_A <@ O1.get(x); sk <@ O2.get(x);}
-      [^match#Some.^match#Pending.^if - ^sk<-] -
-    ]
-
-    proc c_test [
-      ^if.^match#Some.^match#Accepted.^if.^if.^k<- ~ {ks <$ dkey; k <- Some ks;}
-      ^if.^match#Some.^match#Accepted.^if.^if.^c_smap<- ~ {c_smap.[i] <- set_ir_test (Accepted st' t' ks ir');}
-    ]
-
-    proc s_test [
-      ^if.^match#Some.^match#Accepted.^if.^if.^k<- ~ {ks <$ dkey; k <- Some ks;}
-      ^if.^match#Some.^match#Accepted.^if.^if.^s_smap<- ~ {s_smap.[(b, j)] <- set_ir_test (Accepted st' t' ks ir');}
-    ]
-  }
-
-  proc distinguish() = {
-    var b;
-    AKE_O.init_mem(false);
-    b <@ D(AKE_O).run();
-    return b;
-  }
-}.
-
-print Red_ROM4_real.AKE_O.
+print Red_ROM2_real.AKE_O.
 
 (* ------------------------------------------------------------------------------------------ *)
 (* Security Proof *)
 (* ------------------------------------------------------------------------------------------ *)
 section.
 
-declare module A <: A_GAKE {-GAKEb, -Game0, -Game1, -Game2, -Game3, (*-Game4, -Game5, -No_Bad_Game,*) -ROc.IdealAll.RO, -RO, -FRO, -ROSc.I1.RO, -ROSc.I2.RO, -ROSc.I1.FRO, -ROSc.I2.FRO, -Red_Coll_real, -Red_Coll_ideal, -BB.Sample, -Red_ROM_real, -Red_ROM_ideal, -Red_ROM2_real, -Red_ROM_ideal }.
+declare module A <: A_GAKE {-GAKEb, -Game0, -Game1, -Game2, -Game3, -ROc.IdealAll.RO, -RO, -FRO, -ROSc.I1.RO, -ROSc.I2.RO, -ROSc.I1.FRO, -ROSc.I2.FRO, -Red_Coll_real, -Red_Coll_ideal, -BB.Sample, -Red_ROM_real, -Red_ROM_ideal, -Red_ROM2_real, -Red_ROM3_real }.
 
 declare axiom A_ll (G <: GAKE_out{-A}):
   islossless G.h =>
@@ -661,7 +618,6 @@ smt(in_fset0).
 qed.
 
 
-
 (* ------------------------------------------------------------------------------------------ *)
 (* Step 1: Remove collisions in ephemeral and long-term keys. Strategy with single birthday bound. *)
 lemma game0_musplit bit &m: Pr[E_GAKE(Game0, A).run(bit) @ &m : res] = Pr[E_GAKE(Game0, A).run(bit) @ &m : res /\ Game0.bad] + Pr[E_GAKE(Game0, A).run(bit) @ &m : res /\ !Game0.bad]. 
@@ -876,7 +832,7 @@ local clone import DProd.ProdSampling with
   type t2 <- key
 proof *.
 
-lemma game1_splitRO bit &m: Pr[E_GAKE(Game1, A).run(bit) @ &m : res] =  Pr[E_GAKE(Game2, A).run(bit) @ &m : res].
+lemma game1_game2 bit &m: Pr[E_GAKE(Game1, A).run(bit) @ &m : res] =  Pr[E_GAKE(Game2, A).run(bit) @ &m : res].
 proof.
 case (bit = false) => real_ideal.
 
@@ -1012,9 +968,12 @@ smt(emptyE).
 qed.
 
 
+
+
+
+
 (* ------------------------------------------------------------------------------------------ *)
 (* Step 3: Moving sampling of the shared key. *)
-
 
 lemma game2_game3_ideal &m: Pr[E_GAKE(Game2, A).run(true) @ &m : res] = Pr[E_GAKE(Game3, A).run(true) @ &m : res].
 proof.
@@ -1042,6 +1001,34 @@ call (: ={b0, hm, servers, c_smap, s_smap, tested, kp_set, bad, h1m, h2m, hq, tq
 
 auto => />.
 qed. 
+
+lemma game3_real_ideal &m: Pr[E_GAKE(Game3, A).run(false) @ &m : res] = Pr[E_GAKE(Game3, A).run(true) @ &m : res].
+proof.
+byequiv => //.
+proc; inline. 
+call (: ={hm, servers, c_smap, s_smap, tested, kp_set, bad, h1m, h2m, hq, tq, badq}(Game3, Game3) /\ Game3.b0{1} = false /\ Game3.b0{2} = true); 1..11: sim />. 
+
++ proc; inline.
+  sp; if => //.
+  match = => // st.
+  match = => // st' pt' k' ir'.
+  if => //.
+  rcondt{1} ^if. auto.
+  rcondf{2} ^if. auto.
+  auto => />.
+
++ proc; inline.
+  sp; if => //.
+  match = => // st.
+  match = => // st' pt' k' ir'.
+  if => //.
+  rcondt{1} ^if. auto.
+  rcondf{2} ^if. auto.
+  auto => />.
+
+auto => />.
+qed. 
+
 
 
 (* Clearing the key out of the state *)
@@ -1341,273 +1328,28 @@ oget ROSc.I2.RO.m{2}.[m3{2}.`1 ^ sk_ce{2}, pk_b{2} ^ sk_ce{2}, b{2}, pk_ce{2}, m
     smt(get_setE).
 qed.
 
-
-
-
-
-
-
-
-
-
-
-lemma splitRO_game2_real &m: Pr[ROc.IdealAll.MainD(Red_ROM_real(A), ROSc.RO_Pair(ROSc.I1.RO,ROSc.I2.RO)).distinguish() @ &m : res] = Pr[E_GAKE(Game2, A).run(false) @ &m : res].
-proof.
-byequiv (: ={glob A, glob Red_ROM2_real} /\ arg{2} = false ==> _)  => //.
+lemma game3_delay_real &m: Pr[E_GAKE(Game3, A).run(false) @ &m : res] = Pr[ROSc.I2.MainD(Red_ROM3_real(A, ROSc.I1.RO), ROSc.I2.RO).distinguish() @ &m : res].
+proof. 
+byequiv => //.
 proc*.
-
-outline {1} [1] { r <@ ROSc.I2.MainD(Red_ROM2_real(A, ROSc.I1.RO), ROSc.I2.RO).distinguish(); }.
-
-+ inline*; wp.
-  call (: ={b0, hm, servers, c_smap, s_smap, tested, kp_set, bad}(Red_ROM_real.AKE_O, Red_ROM2_real.AKE_O) /\ ={ROSc.I1.RO.m, ROSc.I2.RO.m}
-          /\ (forall i st pt k ir, Red_ROM_real.AKE_O.c_smap{1}.[i] = Some (Accepted st pt k ir)
-                => (exists k', Red_ROM2_real.AKE_O.c_smap{2}.[i] = Some (Accepted st pt k' ir))
-                   /\ ((oget pt.`2).`1 ^ st.`4, st.`2 ^ st.`4, st.`1, st.`3, (oget pt.`2).`1) \in ROSc.I2.RO.m{2}
-                   /\ k = oget ROSc.I2.RO.m{2}.[((oget pt.`2).`1 ^ st.`4, st.`2 ^ st.`4, st.`1, st.`3, (oget pt.`2).`1)])
-          /\ (forall i st pt k ir, Red_ROM_real.AKE_O.s_smap{1}.[i] = Some (Accepted st pt k ir)
-                => (exists k', Red_ROM2_real.AKE_O.s_smap{2}.[i] = Some (Accepted st pt k' ir))
-                   /\ (pt.`1 ^ oget st.`3, pt.`1 ^ st.`2, st.`1, pt.`1, (oget pt.`2).`1) \in ROSc.I2.RO.m{2}
-                   /\ k = oget ROSc.I2.RO.m{2}.[(pt.`1 ^ oget st.`3, pt.`1 ^ st.`2, st.`1, pt.`1, (oget pt.`2).`1)])
-
-          /\ forall x, x \in ROSc.I1.RO.m{1} <=> x \in ROSc.I2.RO.m{1}); last first.
-  - by auto => />; smt(map_empty emptyE).
-
-  - proc; inline; auto => />; smt(mem_set get_setE).
-
-  - by sim />. 
-  
-  - by sim />.
-
-  - proc; inline.
-    sp; if => //.
-    sp; match.
-    + smt().
-    + smt().
-    + by auto=> />; smt(get_setE).
-    move=> stl str; auto=> />.
-    smt(get_setE).
-
-  - proc; inline.
-    sp; match = => // sk.
-    match => //.
-    seq 1 1: (#pre /\ ={kp}); 1:by auto.
-    sp 1 1; if => //.
-    swap {1} ^r0<$ @ 1; swap {1} ^r3<$ @ 2.
-    swap {2} ^r0<$ @ 1; swap {2} ^r1<$ @ 2. 
-    seq  2  2: (#pre /\ ={r0} /\ r3{1} = r1{2}); 1: by auto=> />.
-    sp 4 3; if {1} => //.
-    + rcondt {1} ^if; 1: by auto => /#.
-      rcondt {2} ^if; 1: by auto => /#.
-      rcondt {2} ^if; 1: by auto => /#. 
-      auto => /> &1. 
-      smt(mem_set get_setE).
-    rcondf {1} ^if; 1: by auto => /#.
-    rcondf {2} ^if; 1: by auto => /#.
-    rcondf {2} ^if; 1: by auto => /#.
-    auto => /> &2. admit.
-
-  - proc; inline.
-    sp; match=> // stl str.
-    match => // st'l ptl irl st'r ptr irr.
-    swap {1} ^r0<$ @ 1; swap {1} ^r3<$ @ 2.
-    swap {2} ^r0<$ @ 1; swap {2} ^r1<$ @ 2.
-    seq  2  2: (#pre /\ ={r0} /\ r3{1} = r1{2}); 1: by auto.
-    sp ^if & -1   ^if & -1.
-    if{1} => //.
-    + rcondt {1} ^if; 1: by auto => /#.
-      rcondt {2} ^if; 1: by auto => /#.
-      rcondt {2} ^if; 1: by auto => /#. 
-      auto => /> &1. 
-      smt(mem_set get_setE).
-    rcondf {1} ^if; 1: by auto => /#.
-    rcondf {2} ^if; 1: by auto => /#.
-    rcondf {2} ^if; 1: by auto => /#.
-    auto => /> &1 &2. 
-    smt(mem_set get_setE). 
-
-  - proc; inline.
-    sp; match=> // stl str.
-    match => // st'l ptl kl irl st'r ptr kr irr.
-    if => //; auto=> />; smt(get_setE mem_set).
-
-  - proc; inline.
-    sp; match=> // stl str.
-    match => // st'l ptl kl irl st'r ptr kr irr.
-    if => //; auto=> />; smt(get_setE mem_set).
-
-  - proc; inline.
-    sp; match=> // stl str.
-    match => // kpl kpr.
-    if => //; auto=> />. 
-    by smt(get_setE mem_set).
-
-  - proc; inline.
-    sp; match=> // stl str.
-    match => // st'l ptl irl st'r ptr irr.
-    + if => //; auto=> />; smt(get_setE mem_set).
-    move => k ir.
-    if => //; auto => />; smt(get_setE mem_set).
-
-  - proc; inline.
-    sp; match=> // stl str.
-    match => // st'l ptl irl st'r ptr irr k ir.
-    if => //; auto => />; smt(get_setE mem_set).
-
-  - proc; inline.
-    sp; if => //; match=> // stl str.
-    match => // st'l ptl kl irl st'r ptr kr irr.
-    if => //; 1: auto=> /#.
-    if => //; auto => />. 
-    + smt(get_setE mem_set).
-    move => &2 *.
-    split. smt().
-    move => i0 st pt k0 ir. 
-    move => H. split. 
-    case (i0 = i{2}) => i0i.
-    rewrite i0i !get_set_sameE.
-    move => H.
-    split. smt().
-    split. 
-    smt(get_setE mem_set).
-    admit.
-    
-
-  - proc; inline.
-    sp; if => //; match=> // stl str.
-    match => // st'l ptl irl st'r ptr irr k' ir'.
-    if => //; 1: auto=> /#.
-    if => //; auto => />. 
-    + smt(get_setE mem_set).
-    admit.
-
-admit. 
-qed.
- 
-
-
-
-
-
-
-(* old code
-
-
-(* Clearing the key out of the state *)
-local op s_clear_k (s : pr_st_server instance_state) =
-match s with
-| Pending _ _ _ => s
-| Accepted st t k ir => if ir.`2 \/ ir.`3 then s else Accepted st t witness ir
-| Aborted _ _ _ => s
-end.
-
-local op c_clear_k (s : pr_st_client instance_state) =
-match s with
-| Pending _ _ _ => s
-| Accepted st t k ir => if ir.`2 \/ ir.`3 then s else Accepted st t witness ir
-| Aborted _ _ _ => s
-end.
-
-(* Equivalence of partnering notions after keys are cleared *)
-local lemma c_eq_partners_ck tr sml smr: 
-  (forall h, omap (fun (v: pr_st_server instance_state) => s_clear_k v) sml.[h] = smr.[h]) =>
-untested_partner_c tr sml = untested_partner_c tr smr.
-proof.
-move=> eqsm @/untested_partner_c.
-have ->: get_partners_c tr sml = get_partners_c tr smr.
-+ rewrite /get_partners_c; apply: fsetP=> x; rewrite !mem_fdom.
-  rewrite !mem_filter !domE -eqsm.
-  by case: (sml.[x])=> /> [] @/s_clear_k /#.
-have -> //: get_untested_partners_c tr sml = get_untested_partners_c tr smr.
-rewrite /get_untested_partners_c; apply: fsetP=> x; rewrite !mem_fdom.
-rewrite !mem_filter !domE -eqsm.
-by case: (sml.[x])=> /> [] @/s_clear_k /#.
-qed.
-
-local lemma s_eq_partners_ck tr sml smr: 
-  (forall h, omap (fun (v: pr_st_client instance_state) => c_clear_k v) sml.[h] = smr.[h]) =>
-untested_partner_s tr sml = untested_partner_s tr smr.
-proof.
-move=> eqsm @/untested_partner_s.
-have ->: get_partners_s tr sml = get_partners_s tr smr.
-+ rewrite /get_partners_s; apply: fsetP=> x; rewrite !mem_fdom.
-  rewrite !mem_filter !domE -eqsm.
-  by case: (sml.[x])=> /> [] @/c_clear_k /#.
-have -> //: get_untested_partners_s tr sml = get_untested_partners_s tr smr.
-rewrite /get_untested_partners_s; apply: fsetP=> x; rewrite !mem_fdom.
-rewrite !mem_filter !domE -eqsm.
-by case: (sml.[x])=> /> [] @/c_clear_k /#.
-qed.
-
-local lemma c_eq_origins_ck tr sml smr: 
-  (forall h, omap (fun (v: pr_st_server instance_state) => s_clear_k v) sml.[h] = smr.[h]) =>
-untested_origins_c tr sml = untested_origins_c tr smr.
-proof.
-move=> eqsm; rewrite /untested_origins_c.
-have ->: get_origins_c tr sml = get_origins_c tr smr.
-+ rewrite /get_origins_c; apply: fsetP=> x; rewrite !mem_fdom.
-  rewrite !mem_filter !domE -eqsm.
-  by case: (sml.[x])=> /> [] @/s_clear_k /#.
-have -> //: get_untested_origins_c tr sml = get_untested_origins_c tr smr.
-rewrite /get_untested_origins_c; apply: fsetP=> x; rewrite !mem_fdom.
-rewrite !mem_filter !domE -eqsm.
-by case: (sml.[x])=> /> [] @/s_clear_k /#.
-qed.
-
-local lemma c_eq_fresh_ck tr sm1l sm1r sm2: 
-  (forall h, omap (fun (v: pr_st_server instance_state) => s_clear_k v) sm1l.[h] = sm1r.[h]) =>
-fresh_partner_c tr sm1l sm2 = fresh_partner_c tr sm1r sm2.
-proof.
-move=> eqsm; rewrite /fresh_partner_c.
-have ->: get_fresh_partners_c tr sm1l sm2 = get_fresh_partners_c tr sm1r sm2.
-+ rewrite /get_fresh_partners_c; apply: fsetP=> x; rewrite !mem_fdom.
-  rewrite !mem_filter !domE -eqsm.
-  by case: (sm1l.[x])=> /> [] @/s_clear_k /#.
-have -> //: get_origins_c tr sm1l = get_origins_c tr sm1r.
-rewrite /get_origins_c; apply: fsetP=> x; rewrite !mem_fdom.
-rewrite !mem_filter !domE -eqsm.
-by case: (sm1l.[x])=> /> [] @/s_clear_k /#.
-qed.
-
-local lemma s_eq_fresh_ck tr sml smr: 
-  (forall h, omap (fun (v: pr_st_client instance_state) => c_clear_k v) sml.[h] = smr.[h]) =>
-fresh_partner_s tr sml = fresh_partner_s tr smr.
-proof.
-move=> eqsm; rewrite /fresh_partner_s.
-have ->: get_fresh_partners_s tr sml = get_fresh_partners_s tr smr.
-+ rewrite /get_fresh_partners_s; apply: fsetP=> x; rewrite !mem_fdom.
-  rewrite !mem_filter !domE -eqsm.
-  by case: (sml.[x])=> /> [] @/c_clear_k /#.
-have -> //: get_origins_s tr sml = get_origins_s tr smr.
-rewrite /get_origins_s; apply: fsetP=> x; rewrite !mem_fdom.
-rewrite !mem_filter !domE -eqsm.
-by case: (sml.[x])=> /> [] @/c_clear_k /#.
-qed.
-
-
-lemma splitRO_game2_real &m: Pr[ROc.IdealAll.MainD(Red_ROM_real(A), ROSc.RO_Pair(ROSc.I1.RO,ROSc.I2.RO)).distinguish() @ &m : res] = Pr[E_GAKE(Game2, A).run(false) @ &m : res].
-proof.
-byequiv (: ={glob A, glob Red_ROM2_real} /\ arg{2} = false ==> _)  => //.
-proc*.
-
-outline {1} [1] { r <@ ROSc.I2.MainD(Red_ROM2_real(A, ROSc.I1.RO), ROSc.I2.RO).distinguish(); }.
-
-+ inline*; wp.
-  call (: ={b0, hm, servers, tested, kp_set, bad}(Red_ROM_real.AKE_O, Red_ROM2_real.AKE_O) /\ ={ROSc.I1.RO.m, ROSc.I2.RO.m}
-          /\ (forall h, omap (fun v => c_clear_k v) Red_ROM_real.AKE_O.c_smap.[h]{1} = Red_ROM2_real.AKE_O.c_smap.[h]{2})
-          /\ (forall h, omap (fun v => s_clear_k v) Red_ROM_real.AKE_O.s_smap.[h]{1} = Red_ROM2_real.AKE_O.s_smap.[h]{2})
-          /\ (forall i st pt ir, Red_ROM_real.AKE_O.c_smap{1}.[i] = Some (Pending st pt ir) 
++ inline; wp.
+  call (: ={b0, hm, servers, tested, kp_set, bad, hq, tq, badq}(Game3, Red_ROM3_real.AKE_O) /\ Game3.b0{1} = false
+          /\ Game3.h1m{1} = ROSc.I1.RO.m{2} /\ Game3.h2m{1} = ROSc.I2.RO.m{2}
+          /\ (forall h, omap (fun v => c_clear_k v) Game3.c_smap.[h]{1} = Red_ROM3_real.AKE_O.c_smap.[h]{2})
+          /\ (forall h, omap (fun v => s_clear_k v) Game3.s_smap.[h]{1} = Red_ROM3_real.AKE_O.s_smap.[h]{2})
+          /\ (forall i st pt ir, Game3.c_smap{1}.[i] = Some (Pending st pt ir) 
                 => (exists b, ir = (b, false, false)))
-          /\ (forall i st pt ir, Red_ROM_real.AKE_O.s_smap{1}.[i] = Some (Pending st pt ir) 
+          /\ (forall i st pt ir, Game3.s_smap{1}.[i] = Some (Pending st pt ir) 
                 => ir = (false, false, false))
-          /\ (forall i st pt k ir, Red_ROM_real.AKE_O.c_smap{1}.[i] = Some (Accepted st pt k ir)
-                => (exists k', Red_ROM2_real.AKE_O.c_smap{2}.[i] = Some (Accepted st pt k' ir))
+          /\ (forall i st pt k ir, Game3.c_smap{1}.[i] = Some (Accepted st pt k ir)
+                => (exists k', Red_ROM3_real.AKE_O.c_smap{2}.[i] = Some (Accepted st pt k' ir))
                    /\ ((oget pt.`2).`1 ^ st.`4, st.`2 ^ st.`4, st.`1, st.`3, (oget pt.`2).`1) \in ROSc.I2.RO.m{2}
                    /\ k = oget ROSc.I2.RO.m{2}.[((oget pt.`2).`1 ^ st.`4, st.`2 ^ st.`4, st.`1, st.`3, (oget pt.`2).`1)])
-          /\ (forall i st pt k ir, Red_ROM_real.AKE_O.s_smap{1}.[i] = Some (Accepted st pt k ir)
-                => (exists k', Red_ROM2_real.AKE_O.s_smap{2}.[i] = Some (Accepted st pt k' ir))
+          /\ (forall i st pt k ir, Game3.s_smap{1}.[i] = Some (Accepted st pt k ir)
+                => (exists k', Red_ROM3_real.AKE_O.s_smap{2}.[i] = Some (Accepted st pt k' ir))
                    /\ (pt.`1 ^ oget st.`3, pt.`1 ^ st.`2, st.`1, pt.`1, (oget pt.`2).`1) \in ROSc.I2.RO.m{2}
                    /\ k = oget ROSc.I2.RO.m{2}.[(pt.`1 ^ oget st.`3, pt.`1 ^ st.`2, st.`1, pt.`1, (oget pt.`2).`1)])
-          /\ forall x, x \in ROSc.I1.RO.m{1} <=> x \in ROSc.I2.RO.m{1}); last first.
+          /\ forall x, x \in ROSc.I1.RO.m{2} <=> x \in ROSc.I2.RO.m{2}); last first.
   - by auto => />; smt(map_empty emptyE).
 
   - proc; inline; auto => />; smt(mem_set get_setE).
@@ -1632,19 +1374,15 @@ outline {1} [1] { r <@ ROSc.I2.MainD(Red_ROM2_real(A, ROSc.I1.RO), ROSc.I2.RO).d
     + smt().
     seq 1 1: (#pre /\ ={kp}); 1:by auto.
     sp 1 1; if => //.
-    swap {1} ^r0<$ @ 1; swap {1} ^r3<$ @ 2.
+    swap {1} ^ts<$ @ 1; swap {1} ^ks<$ @ 2.
     swap {2} ^r0<$ @ 1; swap {2} ^r1<$ @ 2. 
-    seq  2  2: (#pre /\ ={r0} /\ r3{1} = r1{2}); 1: by auto=> />.
-    sp 4 3; if {1} => //.
+    seq  2  2: (#pre /\ ts{1} = r0{2} /\ ks{1} = r1{2}); 1: by auto=> />.
+    sp ^if & -1 ^if & -1; if {1} => //.
       + rcondt {1} ^if; 1: by auto => /#.
         rcondt {2} ^if; 1: by auto => /#.
         rcondt {2} ^if; 1: by auto => /#. 
         auto => /> &1 &2.
-        move => *.
-        split. rewrite get_setE //=. move => h.
-        case (h = (b, j){2}) => hbj.
-        rewrite hbj !get_set_sameE //=. 
-        smt(mem_set get_set_sameE).
+        smt(mem_set get_setE).
       + rcondf {1} ^if; 1: by auto => /#.
         rcondf {2} ^if; 1: by auto => /#.
         rcondf {2} ^if; 1: by auto => /#.
@@ -1658,9 +1396,9 @@ outline {1} [1] { r <@ ROSc.I2.MainD(Red_ROM2_real(A, ROSc.I1.RO), ROSc.I2.RO).d
     move=> stl str.
     match => //; 1..3: smt().
     move => st'l ptl irl st'r ptr irr.
-    swap {1} ^r0<$ @ 1; swap {1} ^r3<$ @ 2.
+    swap {1} ^ts<$ @ 1; swap {1} ^ks<$ @ 2.
     swap {2} ^r0<$ @ 1; swap {2} ^r1<$ @ 2.
-    seq  2  2: (#pre /\ ={r0} /\ r3{1} = r1{2}); 1: by auto.
+    seq  2  2: (#pre /\ ts{1} = r0{2} /\ ks{1} = r1{2}); 1: by auto.
     sp ^if & -1   ^if & -1.
     seq  ^if{3} & -1   ^if{3} & -1: (#pre /\ ={t_A} /\ sk{2} = witness /\ (x0{2} \in ROSc.I1.RO.m{2}) /\ sk{1} =
 oget ROSc.I2.RO.m{2}.[m3{2}.`1 ^ sk_ce{2}, pk_b{2} ^ sk_ce{2}, b{2}, pk_ce{2}, m3{2}.`1]).
@@ -1675,21 +1413,21 @@ oget ROSc.I2.RO.m{2}.[m3{2}.`1 ^ sk_ce{2}, pk_b{2} ^ sk_ce{2}, b{2}, pk_ce{2}, m
         by auto=> />; smt(mem_set get_setE).
     if=> //. 
     + auto=> /> &1 &2.
-      case _: (Red_ROM.AKE_O.c_smap{1}.[i{2}])=> /> c_smap1_i.
-      case _: (Red_ROM2.AKE_O.c_smap.[i]{2})=> /> c_smap2_i.
+      case _: (Game3.c_smap{1}.[i{2}])=> /> c_smap1_i.
+      case _: (Red_ROM3_real.AKE_O.c_smap.[i]{2})=> /> c_smap2_i.
       move=> c_clear s_clear inv1 inv2 inv3 inv4 eq_dom mem_ro.
       move: c_smap2_i; rewrite -c_clear.
       rewrite c_smap1_i=> />. 
       smt(get_setE).
     + auto=> /> &1 &2.
-      case _: (Red_ROM.AKE_O.c_smap{1}.[i{2}])=> /> c_smap1_i.
-      case _: (Red_ROM2.AKE_O.c_smap.[i]{2})=> /> c_smap2_i.
+      case _: (Game3.c_smap{1}.[i{2}])=> /> c_smap1_i.
+      case _: (Red_ROM3_real.AKE_O.c_smap.[i]{2})=> /> c_smap2_i.
       move=> c_clear s_clear inv1 inv2 inv3 eq_dom mem_ro.
       move: c_smap2_i; rewrite -c_clear.
       rewrite c_smap1_i=> />.
       by smt(get_setE).
 
-  - proc; inline.
+- proc; inline.
     sp; match=> //.
     + smt().
     + smt().
@@ -1700,8 +1438,8 @@ oget ROSc.I2.RO.m{2}.[m3{2}.`1 ^ sk_ce{2}, pk_b{2} ^ sk_ce{2}, b{2}, pk_ce{2}, m
     + auto=> />. smt(c_eq_partners_ck).
     rcondf{2} ^if; 1: by auto => /#.
     auto => /> &1 &2.
-    case _: (Red_ROM.AKE_O.c_smap{1}.[i{2}])=> /> c_smap1_i.
-    case _: (Red_ROM2.AKE_O.c_smap.[i]{2})=> /> c_smap2_i.
+    case _: (Game3.c_smap{1}.[i{2}])=> /> c_smap1_i.
+    case _: (Red_ROM3_real.AKE_O.c_smap.[i]{2})=> /> c_smap2_i.
     move=> c_clear s_clear inv1 inv2 inv3 inv4 eq_dom _ k _. 
     smt(get_setE mem_set).
 
@@ -1716,12 +1454,12 @@ oget ROSc.I2.RO.m{2}.[m3{2}.`1 ^ sk_ce{2}, pk_b{2} ^ sk_ce{2}, b{2}, pk_ce{2}, m
     + auto=> />. smt(s_eq_partners_ck).
     rcondf{2} ^if; 1: by auto => /#.
     auto => /> &1 &2.
-    case _: (Red_ROM.AKE_O.s_smap{1}.[(b, j){2}])=> /> s_smap1_i.
-    case _: (Red_ROM2.AKE_O.s_smap.[(b, j)]{2})=> /> s_smap2_i.
+    case _: (Game3.s_smap{1}.[(b, j){2}])=> /> s_smap1_i.
+    case _: (Red_ROM3_real.AKE_O.s_smap.[(b, j)]{2})=> /> s_smap2_i.
     move=> c_clear s_clear inv1 inv2 inv3 inv4 eq_dom _ k _.
     smt(get_setE mem_set).
-  
-  - proc; inline.
+
+- proc; inline.
     sp; match => //.
     move => stl str.
     match = => // kp.
@@ -1730,11 +1468,11 @@ oget ROSc.I2.RO.m{2}.[m3{2}.`1 ^ sk_ce{2}, pk_b{2} ^ sk_ce{2}, b{2}, pk_ce{2}, m
       split.
       + move => + j - /(_ j). 
         rewrite !domE -s_clear => />.
-        case : (Red_ROM.AKE_O.s_smap.[b{2}, j]{1}) => />.
+        case : (Game3.s_smap.[b{2}, j]{1}) => />.
         smt(s_eq_partners_ck). 
       move => + j - /(_ j). 
       rewrite !domE -s_clear => />.
-      case : (Red_ROM.AKE_O.s_smap.[b{2}, j]{1}) => />.
+      case : (Game3.s_smap.[b{2}, j]{1}) => />.
       smt(s_eq_partners_ck).
     auto => />.
   
@@ -1753,7 +1491,7 @@ oget ROSc.I2.RO.m{2}.[m3{2}.`1 ^ sk_ce{2}, pk_b{2} ^ sk_ce{2}, b{2}, pk_ce{2}, m
     auto => /> &1 &2.
     smt(get_setE).
 
-  - proc; inline.
+- proc; inline.
     sp; match => //.
     + smt().
     + smt().
@@ -1772,11 +1510,13 @@ oget ROSc.I2.RO.m{2}.[m3{2}.`1 ^ sk_ce{2}, pk_b{2} ^ sk_ce{2}, b{2}, pk_ce{2}, m
     move => stl str.
     match => //; 1..3: smt().
     move => st'l ptl kl irl st'r ptr kr irr.
-    if => //.
+    if => //. 
     + auto => />.
       smt(c_eq_fresh_ck).
-    auto => />.
-    smt(get_setE).
+    rcondt{1} ^if; 1: by auto.
+    rcondt{2} ^if; 1: by auto.
+    auto => /> &1 &2 *. 
+    admit. (* add in invariant that in tested case we don't care about value of key *)
 
   - proc; inline.
     sp; if => //; sp; match => //.
@@ -1788,60 +1528,183 @@ oget ROSc.I2.RO.m{2}.[m3{2}.`1 ^ sk_ce{2}, pk_b{2} ^ sk_ce{2}, b{2}, pk_ce{2}, m
     if => //.
     + auto => />.
       smt(s_eq_fresh_ck).
+    rcondt{1} ^if; 1: by auto.
+    rcondt{2} ^if; 1: by auto.
     auto => />.
-    smt(get_setE).
-
-have ll : forall (c : pkey * pkey * s_id * pkey * pkey), is_lossless dkey by move=> _; exact dkey_ll.
-rewrite equiv [{1} 1 (ROSc.I2.FullEager.RO_LRO (Red_ROM2(A, ROSc.I1.RO)) ll)].
-
-inline; wp. 
-call (: ={hm, servers, c_smap, s_smap, tested, kp_set, bad}(Red_ROM2.AKE_O, Game2) /\ ROSc.I1.RO.m{1} = Game2.h1m{2} /\ ROSc.I2.RO.m{1} = Game2.h2m{2});
- try sim />.
-
-- by proc; inline; auto => />.
-
-- proc; inline.
-  sp. match = => // sk.
-  match = => //.
-  seq 1 1: (#pre /\ ={kp}); 1: by auto.
-  sp 1 1; if => //.
-  sp; seq 1 1: (#pre /\ r0{1} = ts{2}); 1: by auto => />.
-  auto => />.
-
-- proc; inline.
-  sp. match = => // st.
-  match = => // st' pt' ir'. 
-  auto => />.
-
-- proc; inline.
-  sp; match = => // st.
-  match = => // st' pt' k' ir'.
-  if => //.
-  auto => />. 
-  smt(get_setE mem_set).
-
-- proc; inline.
-  sp; match = => // st.
-  match = => // st' pt' k' ir'.
-  if => //. auto => />.
-  smt(get_setE mem_set).
-
-- proc; inline.
-  sp; if => //. sp; match = => // st.
-  match = => // st' pt' k' ir'.
-  if => //. auto => />.
-  smt(get_setE mem_set).
-
-- proc; inline.
-  sp; if => //. sp; match = => // st.
-  match = => // st' pt' k' ir'.
-  if => //. auto => />.
-  smt(get_setE mem_set).
-
-auto => />.
+    admit. (* add in invariant that in tested case we don't care about value of key *)
 qed.
 
-*)
+
+lemma sofar &m: `| Pr[E_GAKE(GAKEb(NTOR_S(RO), NTOR_C(RO), RO), A).run(false) @ &m : res] - Pr[E_GAKE(GAKEb(NTOR_S(RO), NTOR_C(RO), RO), A).run(true) @ &m : res]|
+  <= `|Pr[ROSc.I2.MainD(Red_ROM2_real(A, ROSc.I1.RO), ROSc.I2.RO).distinguish() @ &m : res] - Pr[ROSc.I2.MainD(Red_ROM3_real(A, ROSc.I1.RO), ROSc.I2.RO).distinguish() @ &m : res]|
+      + 2%r * ((q_is + q_m1 + q_m2) ^ 2)%r * mu1 dkp (mode dkp).
+proof.   
+rewrite !(gake_game0 _).
+apply (StdOrder.RealOrder.ler_trans 
+        (`|Pr[E_GAKE(Game1, A).run(false) @ &m : res] - Pr[E_GAKE(Game1, A).run(true) @ &m : res]| + 2%r * ((q_is + q_m1 + q_m2) ^ 2)%r * mu1 dkp (mode dkp))).
++ smt(game0_game1 game0_bad).
+by rewrite !(game1_game2 _) game2_game3_ideal -game3_real_ideal game2_delay_real game3_delay_real.
+qed. 
+
+
+
+
+
+
+lemma interestingbit &m: `|Pr[ROSc.I2.MainD(Red_ROM2_real(A, ROSc.I1.RO), ROSc.I2.RO).distinguish() @ &m : res] - Pr[ROSc.I2.MainD(Red_ROM3_real(A, ROSc.I1.RO), ROSc.I2.RO).distinguish() @ &m : res]| <= Pr[ROSc.I2.MainD(Red_ROM2_real(A, ROSc.I1.RO), ROSc.I2.RO).distinguish() @ &m : Red_ROM2_real.AKE_O.badq].
+proof.
+rewrite StdOrder.RealOrder.distrC.
+byequiv (: _ ==> _) : Red_ROM3_real.AKE_O.badq => //; first last.
++ smt().
+symmetry; proc; inline.
+wp.
+call (: Red_ROM3_real.AKE_O.badq
+      , ={b0, servers, c_smap, s_smap, tested, kp_set, hm, bad, hq, tq, badq}(Red_ROM2_real.AKE_O, Red_ROM3_real.AKE_O)
+        /\ ROSc.I1.RO.m{1} = ROSc.I1.RO.m{2} /\ ROSc.I2.RO.m{1} = ROSc.I2.RO.m{2}
+      , ={badq}(Red_ROM2_real.AKE_O, Red_ROM3_real.AKE_O)) => //; try sim />.
+
+- exact A_ll.
+
+- proc; inline; auto => />.
+- move => &2 badq; proc*; inline. auto => />. 
+  rewrite dkey_ll dtag_ll //=. admit.
+- move => &1; proc*; inline; auto.
+  rewrite dkey_ll dtag_ll //=. admit.
+
+- move => &2 badq.
+  proc; if; auto.
+  rewrite dkp_ll //=.
+- move => &1. 
+  proc; if => //. 
+  rcondf ^if; auto => />. admit.
+  by rewrite dkp_ll.
+
+- move => &2 badq.
+  proc; auto => />.
+- move => &1. 
+  proc; auto => />. 
+
+- move => &2 bad.
+  proc; sp; if => //; sp. 
+  match; auto => />.
+  + rewrite dkp_ll. smt().
+  by smt().
+- move => &1. 
+  proc; sp; if => //. 
+  sp; match; auto => />.
+  + by rewrite dkp_ll.
+  by smt().
+
+- move => &2 bad.
+  proc; inline; sp; match; auto => />.
+  match; auto => />. 
+  admit.
+- move => &1. 
+  proc; inline; sp; match; auto => />.
+  match; 2: by auto => />. 
+  admit.
+
+- move => &2 bad.
+  proc; inline.
+  sp; match; auto. 
+  match; auto => />.
+  by rewrite dkey_ll dtag_ll.
+- move => &1.
+  proc; inline*; auto => />.
+  sp; match; auto.
+  match; auto.
+  by rewrite dkey_ll dtag_ll.
+
+- move => &2 bad.
+  proc; sp; match; 1: by auto. 
+  match; auto => />.
+  if => //; inline.
+  auto => />.
+  by rewrite dkey_ll.
+- move => &1.
+  proc; sp; match; 1: by auto. 
+  match; auto => />.
+  if => //; inline. 
+  auto => />.
+  by rewrite dkey_ll.
+
+- move => &2 bad.
+  proc; sp; match; 1: by auto. 
+  match; auto => />.
+  if => //; inline.
+  auto => />.
+  by rewrite dkey_ll.
+- move => &1.
+  proc; sp; match; 1: by auto. 
+  match; auto => />.
+  if => //; inline.
+  auto => />.
+  by rewrite dkey_ll.
+
+- move => &2 bad.
+  proc; sp; match; 1: by auto. 
+  match; auto => />.
+- move => &1.
+  proc; sp; match; 1: by auto. 
+  match; auto => />.
+
+- move => &2 bad.
+  proc; sp; match; 1: by auto. 
+  match; auto => />.
+- move => &1.
+  proc; sp; match; 1: by auto. 
+  match; auto => />.
+
+- move => &2 bad.
+  proc; sp; match; 1: by auto. 
+  match; auto => />.
+- move => &1.
+  proc; sp; match; 1: by auto. 
+  match; auto => />.
+
+- admit.
+- move => &2 bad.
+  proc; sp; if => //; sp; match; 1: by auto. 
+  match; auto.
+  if => //; if => //.
+  + inline; auto => />.
+    admit.
+  auto => />.
+  admit.
+- move => &1.
+  proc; sp; if => //; sp; match; 1: by auto. 
+  match; auto.
+  if => //; if => //.
+  + auto => />.
+    admit.
+  auto => />.
+  admit.
+
+- admit.
+- move => &2 bad.
+  proc; sp; if => //; sp; match; 1: by auto. 
+  match; auto.
+  if => //; if => //.
+  + inline; auto => />.
+    admit.
+  auto => />.
+  admit.
+- move => &1.
+  proc; sp; if => //; sp; match; 1: by auto. 
+  match; auto.
+  if => //; if => //.
+  + auto => />.
+    admit.
+  auto => />.
+  admit.
+
+auto => />.
+move => rl rr al bl bql csl hql kpl ssl sl tl tql h1ml h2ml ar br bqr csr hqr kpr ssr sr tr tqr h1mr h2mr. 
+by case : (!bqr) => />.
+qed.
+
+
+
 
 end section.
 
